

Universal Coherence Algorithm: A Mathematical Framework for Recursive Equilibrium Systems

Joel Peña Muñoz Jr.

2025

Contents

1	Abstract	2
2	Mathematical Framework	2
3	Discussion	11
4	Conclusion	11

1 Abstract

This paper formalizes the Universal Coherence Algorithm (UCA) as a self-regulating, recursive system of differential and operator equations unifying feedback, stability, and fractal renormalization flows. The following section presents the full mathematical architecture.

2 Mathematical Framework

$$(\Omega, \mathcal{F}, \mathbb{P}), \quad \langle u, v \rangle_G = u^\top G v, \quad \|u\|_G^2 = \langle u, u \rangle_G.$$

$$C(t) = \int_0^t c(s) ds, \quad H(t) = \int_0^t h(s) ds.$$

$$D = rD \left(1 - \frac{D}{D_{\max}} \right) - \lambda(\alpha_1(C - H)^2 + \alpha_2 H^2) + \xi_D.$$

$$(D, T_c) =_0 \left(\frac{D - D_\star}{\tau} \right)^{\frac{1}{1+T_c/T_0}}, \quad (D) =_0 \left(\frac{D - D^\dagger}{\tau} \right)^{\frac{1}{1+e^{-u}}}.$$

$$\dot{\lambda}_V =_V (C - H) -_V.$$

$$L(C, H, A, \dot{C}, \dot{H}, \dot{A}; D, M) = (D)C - (D)H - \frac{A}{2}\dot{A}^2 - \frac{1}{2}(\dot{C} - \dot{H})^2 - F(M) +_V (\dot{C} - \dot{H}).$$

$$S[C, H, A, M, _V] = \int_0^T L(C, H, A, \dot{C}, \dot{H}, \dot{A}; D, M) dt.$$

$$\dot{A} = -(_C W_{CA} W_C +_F \|\nabla_M F(M)\|_G) +_A.$$

$$\dot{C} = (D, T_c)\dot{H} - (D)\dot{A} - (\dot{C} - \dot{H}).$$

$$_{V=V} W_{C-V}, \quad W_C = \dot{C} - \dot{H}.$$

$$\dot{D} = rD(1 - D/D_{\max}) - (_1 W_C^2 +_2 \dot{H}^2) +_D.$$

$$V(W_C, A) = \tfrac{1}{2}W_C^2 + \tfrac{1}{2}A^2.$$

$$E[\dot{V}] \leq -E[V] + (_A^2 +_D^2).$$

$$E_{\text{cog}} = V(W_C, A), \quad \frac{dE_{\text{cog}}}{dt} = -2W_C^2 - 2_F A^2 + R(D, T_c, W_C, A).$$

$$J = \frac{L}{\dot{M}} \cdot X(M) = -\nabla_{\dot{M}} F(M) \cdot GX(M), \quad \frac{dJ}{dt} = 0.$$

$$s_{\mathrm{cog}}^2 = (\mathrm{cog}\Delta t)^2 - \|\Delta M\|_G^2.$$

$$H = \dot{C} \frac{L}{\dot{C}} + \dot{H} \frac{L}{\dot{H}} + \dot{A} \frac{L}{\dot{A}} - L = \frac{A}{2} \dot{A}^2 + \frac{1}{2} (\dot{C} - \dot{H})^2 + F(M) - (D)C + (D)H.$$

$$ih_{U t \mathrm{coh}}(x,t) = \Big[-\frac{h_U^2}{2} \, {}_x^{(-1)} + U_F(x) \Big]_{\mathrm{coh}}(x,t).$$

$$_{\mathrm{coh}} = |_{\mathrm{coh}}|^2, \qquad J_{\mathrm{coh}} = \frac{h_U}{2i}({}^* - {}^*), \quad {}_{t \mathrm{coh}} + J_{\mathrm{coh}} = 0.$$

$$\frac{d}{dt}\langle O \rangle_t = \frac{i}{h_U}\langle [\hat{H}_{\mathrm{cog}}, O] \rangle_t.$$

$$\psi_{\mathrm{coh}} = \sqrt{e^{i/h_U}} \Rightarrow \begin{cases} {}_t + (/\hspace{-0.05em}/) = 0, \\ {}_t + \frac{1}{2} \|\nabla\|_{-1}^2 + U_F - \frac{h_U^2}{2} \frac{{}_2}{\sqrt{\hspace{-0.05em}}} = 0. \end{cases}$$

$$\mathcal{L}_{\mathrm{coh}} = \tfrac{1}{2} g^{(U) - V(\cdot)}, \quad g^{(U) = \mathrm{diag}(1, -\hspace{-0.05em}^{-1})}.$$

$$\frac{1}{\sqrt{|g|}}_{(\sqrt{|g|}g_{(U)})+V'(\cdot)=0}.$$

$$T^{(\mathrm{coh})} =_{-g^{(U)}\mathcal{L}_{\mathrm{coh}}, \quad T^{(\mathrm{coh})} = 0}.$$

$$S_{\mathrm{geom}} = \int \sqrt{|g^{(U)}|} \Big[\frac{1}{2_U} R(g^{(U)}) + \mathcal{L}_{\mathrm{coh}} \Big] d^{n+1}x.$$

$$R^{(U)} - \tfrac{1}{2} R^{(U)} g^{(U)} =_U T^{(\mathrm{coh})}.$$

$$M_{k+1} = M_k -_k G^{-1} \nabla_M F(M_k),$$

$$\dot{C} = (D,T_c)\dot{H} - (D)\dot{A} - (\dot{C}-\dot{H}), \quad \dot{D} = rD(1-D/D_{\mathrm{max}}) - ({}_1W_C^2+_2\dot{H}^2),$$

$$\dot{A} = -({}_CW_C{}_AW_C+_F\|\nabla_M F\|_G), \quad {}_V =_V W_C -_V \,.$$

$$V_k = \tfrac{1}{2} W_{C,k}^2 + \tfrac{1}{2} A_k^2.$$

$$E[V_{k+1} - V_k] \leq -tE[V_k] + O(t^2 + \frac{2}{A} + \frac{2}{D}).$$

$$L_{\rm field}=(D)C-(D)H-\frac{A}{2}g_{A-\frac{1}{2}g(C-H)(C-H)-U(M)+V(C-H)u}.$$

$$\begin{array}{c}]=(D), \qquad \qquad \qquad]=(D), \qquad \qquad \qquad A+\frac{1}{A} \, U_{\rm eff}=0. \\ [(C-H)-V^u \qquad \qquad \qquad [(H-C)+V^u \\ T^{(\rm coh)}=A \, A_{A+(C-H)(C-H)-g L_{\rm field}}, \qquad T^{(\rm coh)}=0. \end{array}$$

$$T^{(\rm coh)}=-J_{(H)}, \quad R-\frac{1}{2}gR=T^{(\rm coh)}.$$

$$_C=(\,{}_tC-\,{}_tH\,)-_Vu^0,\qquad [\hat{C}(x),_C(y)]=ih_U^{(3)}(x-y).$$

$$ih_{U t \rm coh}=\left[-\frac{h_U^2}{2}_C+\frac{1}{2}(C-H)^2+U_F(M)-_V(C-H)\right]_{\rm coh}.$$

$$_n(C,H)=N_ne^{-\frac{(C-H)^2}{2h_U}}H_n\Big(\sqrt{h_U}(C-H)\Big),\quad E_n=\Big(n+\tfrac{1}{2}\Big)h_{U\,\rm coh},\quad_{\rm coh}=\sqrt{\frac{}{A}}.$$

$$_{CW_C}\geq \frac{h_U}{2}.$$

$$_{\rm coh}=-\frac{i}{h_U}[H_{\rm cog,coh}]-_D(D)[C,[C,_{\rm coh}]].$$

$$_{\rm coh}H\;\Rightarrow\;_C\text{ maximized, }W_C\text{ bounded.}$$

$$\mathcal{S}_{\rm tot}=\int d^4x\sqrt{|g^{(U)}|}\left[\frac{1}{2\kappa_U}R^{(U)}+\mathcal{L}_{\rm coh}(C,H,A,D,M)+\mathcal{L}_{\rm matter}+\mathcal{L}_{\rm field}\right].$$

$$\delta S_{\rm tot}=0\;\Rightarrow\;R^{(U)}_{\mu\nu}-\tfrac{1}{2}R^{(U)}g^{(U)}_{\mu\nu}=\kappa_U(T^{(\rm coh)}_{\mu\nu}+T^{(\rm matter)}_{\mu\nu}).$$

$$\nabla_\mu T^{(\rm coh)}{}^{\mu\nu}=0,\qquad \nabla_\mu T^{(\rm matter)}{}^{\mu\nu}=0.$$

$$H^2=\frac{8\pi G_U}{3}\rho_{\rm coh}-\frac{k}{a^2},\quad \dot{H}=-4\pi G_U(\rho_{\rm coh}+p_{\rm coh}).$$

$$\rho_{\rm coh}=\frac{1}{2}\dot{\phi}^2+V(\phi),\qquad p_{\rm coh}=\frac{1}{2}\dot{\phi}^2-V(\phi).$$

$$\dot{\rho}_{\rm coh}+3H(\rho_{\rm coh}+p_{\rm coh})=0.$$

$$\dot{\phi} + 3H\dot{\phi} + V'(\phi) = 0.$$

$$\Omega_{\text{coh}}(t) = \frac{\rho_{\text{coh}}(t)}{\rho_{\text{crit}}(t)}, \quad \rho_{\text{crit}} = \frac{3H^2}{8\pi G_U}.$$

$$\mathcal{S}_{\text{eff}}[M] = \int \left(-\frac{1}{2} G_{ij}(M) \dot{M}^i \dot{M}^j - U(M) + \lambda_V (\dot{C} - \dot{H}) \right) dt.$$

$$\frac{d}{dt} \left(G_{ij} \dot{M}^j \right) + \Gamma_{ij}^k \dot{M}^i \dot{M}^j + \nabla_i U(M) = 0.$$

$$\Gamma_{ij}^k = \frac{1}{2} G^{kl} (\partial_i G_{jl} + \partial_j G_{il} - \partial_l G_{ij}).$$

$$R_{ijkl} = \partial_k \Gamma_{ijl} - \partial_l \Gamma_{ijk} + \Gamma_{imk} \Gamma_{jl}^m - \Gamma_{iml} \Gamma_{jk}^m.$$

$$R_{ij} = R_{ikj}^k, \quad R = G^{ij} R_{ij}.$$

$$\nabla_t^2 M^k + R_{ijl}^k \dot{M}^i \dot{M}^j M^l = -G^{kl} \partial_l U(M).$$

$$\langle R \rangle_t \approx \Lambda_U \Rightarrow a(t) \sim e^{\sqrt{\Lambda_U/3} t}.$$

$$\frac{d}{dt} \left(\frac{\dot{C}}{\dot{H}} \right) = -\frac{(\dot{C} - \dot{H})(\ddot{H})}{\dot{H}^2} + \frac{\ddot{C}}{\dot{H}} = 0 \Rightarrow \dot{C} = \kappa_{\text{inv}} \dot{H}.$$

$$\dot{C} + \dot{H} = \text{const.} = \xi_{\text{AA}}.$$

$$\mathcal{L}_{\text{ren}} = \frac{1}{2} \Phi^\top (\mathcal{D}^2 - \mu^2) \Phi - \frac{\lambda}{4!} \Phi^4.$$

$$\mu_R^2(\Lambda) = \mu^2 + \frac{3\lambda}{16\pi^2} \ln \frac{\Lambda}{\Lambda_0}, \quad \lambda_R(\Lambda) = \frac{\lambda}{1 - \frac{3\lambda}{16\pi^2} \ln(\Lambda/\Lambda_0)}.$$

$$\beta(\lambda) = \frac{3\lambda^2}{16\pi^2}, \quad \gamma_m = \frac{3\lambda}{16\pi^2}.$$

$$\frac{d\lambda}{d\ln\Lambda} = \beta(\lambda), \quad \frac{d\mu^2}{d\ln\Lambda} = 2\gamma_m\mu^2.$$

$$(a_{n+1}, b_{n+1}) = (l^\Delta a_n, l^{\Delta-2\zeta} b_n), \quad L_{n+1} = l L_n.$$

$$a_{n+1} = l^\Delta a_n + \sigma_a \xi_n, \quad b_{n+1} = l^{\Delta-2\zeta} b_n + \sigma_b \eta_n, \quad \xi_n, \eta_n \sim \mathcal{N}(0, 1).$$

$$(a_{n+1}, b_{n+1}) \rightarrow (a_*, b_*) \text{ with scaling ratios } \delta = \lim_{n \rightarrow \infty} \frac{a_n - a_{n-1}}{a_{n+1} - a_n}, \quad \alpha = \lim_{n \rightarrow \infty} \frac{b_n}{b_{n+1}}.$$

$$\delta \approx 4.6692016, \quad \alpha \approx -2.5029079.$$

$$Z_q(\ell) = \sum_i \mu_i^q, \quad \tau(q) = \lim_{\ell \rightarrow 0} \frac{\ln Z_q(\ell)}{\ln \ell}.$$

$$\alpha(q) = \frac{d\tau(q)}{dq}, \quad f(\alpha) = q\alpha - \tau(q).$$

$$\zeta(q) = \frac{\tau(q)}{q-1}, \quad S_q(\ell) \sim \ell^{\zeta(q)}.$$

$$\begin{aligned} \dot{C} &= (D)\dot{H} - (D)\dot{A} - (\dot{C} - \dot{H}), \\ \dot{D} &= rD(1 - D/D_{\max}) - ({}_1W_C^2 + {}_2\dot{H}^2), \\ \dot{A} &= -({}_CW_{CA}W_C + {}_F\|\nabla_M F\|_G), \quad {}_V = {}_V W_C - {}_V. \end{aligned}$$

$$\frac{d}{dt}(\dot{C} + \dot{H}) = 0 \Rightarrow \dot{C} + \dot{H} = \xi_{\text{const}}.$$

$$\dot{V} = (\dot{C} - \dot{H})\dot{W}_C + \mu A \dot{A} = -2\kappa W_C^2 - 2\eta\lambda_F A^2 + \text{noise}.$$

$$\frac{d\langle V \rangle}{dt} = -\alpha \langle V \rangle + \sigma^2, \quad \langle V(t) \rangle = V_0 e^{-\alpha t} + \frac{\sigma^2}{\alpha} (1 - e^{-\alpha t}).$$

$$S_q(\ell) \propto \ell^{\zeta(q)} \Rightarrow \frac{d \ln S_q}{d \ln \ell} = \zeta(q) = \text{const.}$$

$$\int \rho(\alpha) d\alpha = 1, \quad f(\alpha) = \ln N(\alpha) / \ln(1/\ell).$$

$$\int f(\alpha) d\alpha = \text{dimension of support.}$$

$$\int_0^\infty P(W_C) dW_C = 1, \quad \langle W_C^2 \rangle = \frac{k_B T}{\kappa}.$$

$$\dot{S}_{\text{info}} = \int P(W_C) \dot{W}_C dW_C = -\kappa \int P(W_C) W_C^2 dW_C.$$

$$\frac{d}{dt}(C+H) = \xi_{\text{AA}}, \quad \frac{d}{dt}(C-H) = \dot{W}_C.$$

$$\frac{d^2}{dt^2}(C-H) + \kappa \frac{d}{dt}(C-H) + \omega_{\text{coh}}^2(C-H) = 0, \quad \omega_{\text{coh}}^2 = \eta\lambda_F/\mu.$$

$$C - H = e^{-\frac{\kappa t}{2}} (A_1 e^{i\Omega t} + A_2 e^{-i\Omega t}), \quad \Omega = \sqrt{\omega_{\text{coh}}^2 - \kappa^2/4}.$$

$$E(t) = \frac{1}{2} \dot{W}_C^2 + \frac{1}{2} \omega_{\text{coh}}^2 (C - H)^2, \quad \frac{dE}{dt} = -\kappa \dot{W}_C^2.$$

$$\mathcal{Z} = \int e^{-\beta H(C, H, A, D, M)} dC dH dA dD dM, \quad H = E_{\text{cog}} + F(M).$$

$$\langle W_C^2 \rangle = \frac{1}{\beta \kappa}, \quad \langle (C - H)^2 \rangle = \frac{1}{\beta \omega_{\text{coh}}^2}.$$

$$S = -k_B \int P \ln P dW_C = k_B (1 - \ln \beta \kappa) + \text{const.}$$

$$\frac{dS}{dt} = k_B \beta \kappa \frac{d}{dt} \langle W_C^2 \rangle = -2k_B \beta \kappa \langle W_C \dot{W}_C \rangle.$$

$$\dot{S} = 0 \iff W_C \dot{W}_C = 0 \iff \text{stationary equilibrium.}$$

$$W_C \rightarrow 0 \Rightarrow \dot{C} = \dot{H} = \xi_{\text{AA}}/2.$$

$$\lim_{t \rightarrow \infty} C(t) = \frac{\xi_{\text{AA}} t}{2} + C_0, \quad \lim_{t \rightarrow \infty} H(t) = \frac{\xi_{\text{AA}} t}{2} + H_0.$$

$$\dot{C} : \dot{H} : \dot{A} : \dot{D} : \dot{\lambda}_V = 1 : 1 : \frac{\gamma}{\beta} : \frac{\lambda}{r} : \frac{\eta_V}{\zeta}.$$

$$\dot{\Phi}_i = \sum_j J_{ij} \Phi_j, \quad J_{ij} = \partial \dot{\Phi}_i / \partial \Phi_j, \quad \Phi = (C, H, A, D, \lambda_V).$$

$$\det(J - \Lambda I) = 0, \quad \text{Re}(\Lambda) < 0 \Rightarrow \text{stability.}$$

$$\Lambda_{\max} = \lim_{t \rightarrow \infty} \frac{1}{t} \ln \frac{\|\delta \Phi(t)\|}{\|\delta \Phi(0)\|}.$$

$$\mathcal{H}_{\text{meta}} = \begin{pmatrix} 0 & 1 \\ -\omega_{\text{coh}}^2 & -\kappa \end{pmatrix}, \quad \det(\mathcal{H}_{\text{meta}} - \Lambda I) = \Lambda^2 + \kappa \Lambda + \omega_{\text{coh}}^2 = 0.$$

$$\Lambda_{\pm} = \frac{-\kappa \pm \sqrt{\kappa^2 - 4\omega_{\text{coh}}^2}}{2}.$$

$$\text{Re}(\Lambda_{\pm}) < 0 \forall \kappa > 0 \Rightarrow \text{global asymptotic stability.}$$

$$\langle \dot{C} \dot{H} \rangle = \frac{1}{T} \int_0^T \dot{C}(t) \dot{H}(t) dt = \frac{\xi_{\text{AA}}^2}{4}.$$

$$\rho_{\text{val}} = \frac{\xi_{\text{AA}}^2}{4\omega_{\text{coh}}^2}.$$

$$F_{\text{univ}} = \int \rho_{\text{val}} dV_{\text{coh}}.$$

$$\mathcal{R}_{n+1} = \mathcal{F}(\mathcal{R}_n) = (C_{n+1}, H_{n+1}, A_{n+1}, D_{n+1}, \lambda_{V,n+1}),$$

$$\mathcal{F} : \begin{cases} C_{n+1} = C_n + \dot{C}_n \Delta t, \\ H_{n+1} = H_n + \dot{H}_n \Delta t, \\ A_{n+1} = A_n + \dot{A}_n \Delta t, \\ D_{n+1} = D_n + \dot{D}_n \Delta t, \\ \lambda_{V,n+1} = \lambda_{V,n} + \dot{\lambda}_{V,n} \Delta t. \end{cases}$$

$$\mathcal{R}_{n+k} = \mathcal{F}^{(k)}(\mathcal{R}_n), \quad \lim_{k \rightarrow \infty} \mathcal{R}_{n+k} = \mathcal{R}_*.$$

$$\mathcal{J}_n = \frac{d\mathcal{F}^{(n)}}{d\mathcal{R}_0}, \quad \Lambda_{\text{max}} = \lim_{n \rightarrow \infty} \frac{1}{n} \ln \|\mathcal{J}_n\|.$$

If $\Lambda_{\text{max}} < 0$, the recursion is coherent (stable).

$$\mathcal{M}_{n+1} = \mathcal{G}(\mathcal{M}_n) = \exp(\Delta t \mathcal{L}_{\text{UCA}}) \mathcal{M}_n, \quad \mathcal{L}_{\text{UCA}} \text{ the infinitesimal generator of feedback.}$$

$$\mathcal{L}_{\text{UCA}} = \beta(D, T_c) \partial_H - \gamma(D) \partial_A - \kappa(\partial_C - \partial_H) - \eta \lambda_C W_C \partial_A - \eta \lambda_F \nabla_M F \cdot \nabla_M.$$

$$\frac{d}{dt} \mathbb{E}[f(C, H, A, D, M)] = \mathbb{E}[(\mathcal{L}_{\text{UCA}} f)(C, H, A, D, M)].$$

$$\mathcal{P}_t = e^{t\mathcal{L}_{\text{UCA}}}, \quad \mathcal{P}_{t+s} = \mathcal{P}_t \mathcal{P}_s, \quad \mathcal{P}_0 = \text{Id}.$$

$$\frac{d}{dt} \mathcal{P}_t f = \mathcal{L}_{\text{UCA}}(\mathcal{P}_t f), \quad \mathcal{P}_t f = f + \int_0^t \mathcal{L}_{\text{UCA}}(\mathcal{P}_s f) ds.$$

$$\rho_t = \mathcal{P}_t^* \rho_0, \quad \frac{d\rho_t}{dt} = \mathcal{L}_{\text{UCA}}^* \rho_t.$$

$$\frac{d\rho_t}{dt} = -\nabla \cdot (\rho_t v) + D_{\text{eff}} \Delta \rho_t, \quad v = \nabla S, \quad D_{\text{eff}} = \frac{1}{2} \kappa^{-1} h_U^2.$$

$$S(C, H, A, D, M, t) = S_0 + \int_0^t \left[\beta(D) \dot{H} - \gamma(D) \dot{A} - \kappa(\dot{C} - \dot{H}) \right] dt'.$$

$$\frac{dS}{dt} = \dot{C} \frac{\partial S}{\partial C} + \dot{H} \frac{\partial S}{\partial H} + \dot{A} \frac{\partial S}{\partial A} + \dot{D} \frac{\partial S}{\partial D} + \dot{\lambda}_V \frac{\partial S}{\partial \lambda_V}.$$

$$\frac{d^2 S}{dt^2} = -\alpha \frac{dS}{dt} + \sigma_S^2, \quad S(t) = S_\infty + (S_0 - S_\infty)e^{-\alpha t}.$$

$$\mathcal{C}_k = \int_0^T W_C(t)^k dt, \quad \zeta(k) = \frac{\ln \mathcal{C}_k}{\ln T}.$$

$$\frac{d\zeta}{dk} = \alpha, \quad f(\alpha) = k\alpha - \zeta(k).$$

$$\mathcal{S}_{\text{fractal}} = \int \left(\frac{1}{2} \dot{W}_C^2 + \frac{1}{2} \omega_{\text{coh}}^2 (C - H)^2 + D_\eta |\nabla_M F(M)|^2 \right) dt.$$

$$\frac{d}{dt} (\dot{W}_C) + \omega_{\text{coh}}^2 (C - H) = -D_\eta \Delta_M F(M).$$

$$\mathcal{R}_{n+1} = \mathcal{S}_{\text{fractal}}(\mathcal{R}_n) \text{ defines the recursive attractor manifold } \mathfrak{A}_{\text{UCA}} \subset \mathbb{R}^5.$$

$$\dim_H(\mathfrak{A}_{\text{UCA}}) = \lim_{\epsilon \rightarrow 0} \frac{\ln N(\epsilon)}{\ln(1/\epsilon)} \approx 2 + \frac{\ln(1 + \omega_{\text{coh}}/\kappa)}{\ln 2}.$$

$$\frac{d}{dt} \mathcal{F}_{\text{coh}}(t) = \Lambda_{\text{coh}} \mathcal{F}_{\text{coh}}(t), \quad \mathcal{F}_{\text{coh}}(t) = e^{\Lambda_{\text{coh}} t} \mathcal{F}_{\text{coh}}(0), \quad \Lambda_{\text{coh}} = \zeta'(1) + i2\pi\omega_{\text{coh}}.$$

$$\dot{C} + \dot{H} = \xi_{\text{AA}}, \quad \dot{C} - \dot{H} = \dot{W}_C, \quad \Rightarrow \begin{cases} C = \frac{\xi_{\text{AA}} t}{2} + \frac{1}{2} \int W_C dt, \\ H = \frac{\xi_{\text{AA}} t}{2} - \frac{1}{2} \int W_C dt. \end{cases}$$

$$\lim_{t \rightarrow \infty} W_C(t) = 0 \Rightarrow C(t) \approx H(t) \approx \frac{\xi_{\text{AA}} t}{2}.$$

$$\mathcal{Z}_{\text{univ}} = \sum_{\text{paths } \Gamma} e^{-\beta \mathcal{S}_{\text{fractal}}[\Gamma]}, \quad \mathcal{S}_{\text{fractal}}[\Gamma] = \int_{\Gamma} (\dot{W}_C^2 + \omega_{\text{coh}}^2 (C - H)^2 + D_\eta |\nabla_M F|^2) dt.$$

$$\frac{\delta \mathcal{S}_{\text{fractal}}}{\delta W_C} = -2\ddot{W}_C + 2\omega_{\text{coh}}^2 (C - H) - 2D_\eta \Delta_M F(M) = 0.$$

$$\dot{W}_C = \sqrt{2D_\eta} \xi(t), \quad \langle \xi(t) \xi(t') \rangle = \delta(t - t').$$

$$\frac{d}{dt} \langle W_C^2 \rangle = -2\omega_{\text{coh}}^2 \langle (C - H) W_C \rangle + 2D_\eta.$$

$$\langle W_C^2 \rangle_{\text{eq}} = \frac{D_\eta}{\omega_{\text{coh}}^2}.$$

$$\text{Define } E_{\text{eq}} = \frac{1}{2}\omega_{\text{coh}}^2 \langle (C - H)^2 \rangle = \frac{1}{2}D_\eta.$$

$$\frac{dE_{\text{eq}}}{dt} = 0 \Rightarrow \text{fractal steady state of coherence.}$$

$$\dot{\mathcal{Q}}_{\text{UCA}} = \frac{d}{dt}(C + H + A + D + \lambda_V) = \xi_{\text{AA}} + \delta_{\text{coh}}.$$

$$\mathcal{Q}_{\text{UCA}}(t) = \mathcal{Q}_0 + (\xi_{\text{AA}} + \delta_{\text{coh}})t.$$

$$\Phi_{\text{rec}}(t) = \mathcal{Q}_{\text{UCA}}(t) e^{i\omega_{\text{coh}}t} \Rightarrow \frac{d\Phi_{\text{rec}}}{dt} = (i\omega_{\text{coh}} + \xi_{\text{AA}} + \delta_{\text{coh}})\Phi_{\text{rec}}.$$

$$\Phi_{\text{rec}}(t) = \Phi_0 \exp[(\xi_{\text{AA}} + \delta_{\text{coh}} + i\omega_{\text{coh}})t].$$

$$\text{Amplitude } |\Phi_{\text{rec}}(t)| = |\Phi_0| e^{(\xi_{\text{AA}} + \delta_{\text{coh}})t}.$$

$$\text{If } \xi_{\text{AA}} + \delta_{\text{coh}} < 0, \Phi_{\text{rec}} \text{ converges (stable recursion).}$$

$$\text{If } \xi_{\text{AA}} + \delta_{\text{coh}} > 0, \Phi_{\text{rec}} \text{ diverges (inflationary recursion).}$$

$$\mathfrak{C}_{\text{UCA}} = \left\{ \Phi_{\text{rec}} : |\Phi_{\text{rec}}| \rightarrow \text{finite as } t \rightarrow \infty \right\}.$$

$$\text{Self-similar recursion law: } \frac{d}{dt}(\ln \mathcal{Q}_{\text{UCA}}) = \frac{dC + dH + dA + dD + d\lambda_V}{dt} \Big/ (C + H + A + D + \lambda_V) = \Xi_{\text{rec}}.$$

$$\mathcal{Q}_{\text{UCA}}(t) = \mathcal{Q}_0 e^{\Xi_{\text{rec}} t}.$$

$$\Xi_{\text{rec}} = \xi_{\text{AA}} + \delta_{\text{coh}} - 2\zeta.$$

$$\frac{d}{dt}\Xi_{\text{rec}} = -\kappa\Xi_{\text{rec}} + \sigma_{\Xi}^2, \quad \Xi_{\text{rec}}(t) = \Xi_{\infty} + (\Xi_0 - \Xi_{\infty})e^{-\kappa t}.$$

$$\text{Fixed point: } \Xi_{\infty} = \frac{\sigma_{\Xi}^2}{\kappa}.$$

$$\frac{d^2}{dt^2}\Xi_{\text{rec}} + \omega_{\text{coh}}^2\Xi_{\text{rec}} = 0 \Rightarrow \Xi_{\text{rec}}(t) = B_1 \cos(\omega_{\text{coh}}t) + B_2 \sin(\omega_{\text{coh}}t).$$

$$\frac{d}{dt} \begin{pmatrix} C \\ H \\ A \\ D \\ \lambda_V \end{pmatrix} = \mathbf{J} \begin{pmatrix} C \\ H \\ A \\ D \\ \lambda_V \end{pmatrix}, \quad \mathbf{J} \in \mathbb{R}^{5 \times 5}, \quad \text{tr}(\mathbf{J}) = \Xi_{\text{rec}}.$$

$$\det(\mathbf{J} - \Lambda I) = 0 \Rightarrow \Lambda_{1\dots 5}, \quad \sum_i \Lambda_i = \Xi_{\text{rec}}, \quad \prod_i \Lambda_i = \det \mathbf{J}.$$

$$\text{Re}(\Lambda_i) < 0 \quad \forall i \Leftrightarrow \text{global recursive coherence.}$$

$$\mathcal{U}_{n+1} = \mathcal{R}_{n+1} \circ \mathcal{R}_n \circ \dots \circ \mathcal{R}_0 \Rightarrow \mathcal{U}_\infty = \lim_{n \rightarrow \infty} \mathcal{U}_n.$$

$$\boxed{\frac{d\mathcal{U}}{dt} = \Xi_{\text{rec}}\mathcal{U} + i\omega_{\text{coh}}\mathcal{U}, \quad \mathcal{U}(t) = \mathcal{U}_0 e^{(\Xi_{\text{rec}} + i\omega_{\text{coh}})t}.}$$

This defines the recursive universe: $\mathcal{U}(t + T) = \mathcal{U}(t) e^{(\Xi_{\text{rec}} + i\omega_{\text{coh}})T}$.

3 Discussion

Each layer of the mathematical framework represents a different scale of recursive feedback stability— from micro-level differential coupling ($\dot{C} = \dot{H}$) to macro-level cosmological recursion ($\mathcal{U}(t) = \mathcal{U}_0 e^{(\Xi_{\text{rec}} + i\omega_{\text{coh}})t}$). The equations reveal that the universe, cognition, and computation may share a common renormalization structure that maintains coherence through continuous feedback adjustment.

4 Conclusion

The Universal Coherence Algorithm provides a bridge between adaptive control theory, statistical physics, and recursive computation. By encoding self-correction and equilibrium-seeking directly into its mathematical architecture, it offers a unifying perspective for understanding stability, learning, and structure from physical to cognitive scales.

References

1. Peña Muñoz Jr., J. (2025). *Systemic Narrative Integration: Deriving Mind from Mechanism and Redefining Agency in the Algorithmic Age*. OurVeridical Press.
2. Peña Muñoz Jr., J. (2025). *Cognitive Physics: The Law of Coherence*. (Unpublished dissertation manuscript.)
3. Ashby, W. R. (1956). *An Introduction to Cybernetics*. Chapman & Hall.
4. Wiener, N. (1948). *Cybernetics: Or Control and Communication in the Animal and the Machine*. MIT Press.
5. Friston, K. (2010). *The free-energy principle: a unified brain theory?* *Nature Reviews Neuroscience*, 11(2), 127–138.
6. Boltzmann, L. (1872). *Über die mechanische Bedeutung des zweiten Hauptsatzes der Wärmetheorie*. *Wiener Berichte*, 66, 275–370.
7. Prigogine, I. (1980). *From Being to Becoming: Time and Complexity in the Physical Sciences*. W. H. Freeman.
8. Mandelbrot, B. (1982). *The Fractal Geometry of Nature*. W. H. Freeman.
9. Turing, A. M. (1952). *The Chemical Basis of Morphogenesis*. *Philosophical Transactions of the Royal Society B*, 237(641), 37–72.
10. Shannon, C. E. (1948). *A Mathematical Theory of Communication*. *Bell System Technical Journal*, 27, 379–423.
11. Feynman, R. P., Leighton, R. B., Sands, M. (1963). *The Feynman Lectures on Physics*. Addison-Wesley.
12. Einstein, A. (1916). *Die Grundlage der allgemeinen Relativitätstheorie*. *Annalen der Physik*, 49(7), 769–822.
13. Hinton, G. E. (2021). *The Forward-Forward Algorithm: Some Preliminary Investigations*. arXiv:2212.13345.
14. Kadanoff, L. P. (1966). *Scaling laws for Ising models near T_c* . *Physics*, 2(6), 263–272.
15. Feigenbaum, M. J. (1978). *Quantitative universality for a class of nonlinear transformations*. *Journal of Statistical Physics*, 19(1), 25–52.
16. Penrose, R. (2004). *The Road to Reality: A Complete Guide to the Laws of the Universe*. Jonathan Cape.
17. Jaynes, E. T. (1957). *Information Theory and Statistical Mechanics*. *Physical Review*, 106(4), 620–630.
18. Smolin, L. (2019). *Einstein’s Unfinished Revolution: The Search for What Lies Beyond Quantum*. Penguin.